src/library/vm/vm_int.h
@@ -5,12 +5,16 @@ Released under Apache 2.0 license as described in the file LICENSE.
 Author: Leonardo de Moura
 */
 #pragma once
+#include <limits>
 #include "library/vm/vm.h"
 
 namespace lean {
 int to_int(vm_obj const & o);
 optional<int> try_to_int(vm_obj const & o);
-int force_to_int(vm_obj const & o, int def);
+int force_to_int(vm_obj const & o, int def = std::numeric_limits<int>::max());
+long to_long(vm_obj const & o);
+optional<long> try_to_long(vm_obj const & o);
+long force_to_long(vm_obj const & o, long def = std::numeric_limits<long>::max());
 void initialize_vm_int();
 void finalize_vm_int();
 }
