tests/lean/ffi.lean
@@ -1,4 +1,5 @@
 import system.io
+import system.foreign
 
 namespace tactic
 
@@ -9,17 +10,19 @@ updateex_env $ λ env, pure $ env.load_foreign_object n str
 
 
 end tactic
-open tactic
+open tactic foreign
 
 def main : unit → unit → unit := λ _, id
-
--- run_cmd file
 
 run_cmd
 do
    unsafe_run_io $ do
    { io.env.get_cwd >>= io.print_ln,
-    (io.cmd { cmd := "make", args := ["some_file.so"] }) >>= io.print_ln },
+     b ← io.fs.dir_exists "vm_dynload",
+     io.env.set_cwd "vm_dynload",
+     b ← io.fs.file_exists "some_file.so",
+     if b then io.fs.remove "some_file.so" else pure (),
+     (io.cmd { cmd := "make", args := ["some_file.so"] }) >>= io.print_ln },
    load_foreign_object `foo "vm_dynload/some_file.so",
    -- bind_foreign_symbol `foo `main 2 "main",
    return ()
@@ -27,8 +30,7 @@ do
 run_cmd trace "\nnext!\n"
 
 @[ffi foo]
-constant my_fun : unsigned → unsigned → unsigned
+constant my_fun : uint_32 → int_64 → int_64
 
-run_cmd trace "\nnext!\n"
 
 #eval my_fun 7 3
